PREFIX : <http://www.semanticweb.org/timo.homburg/ontologies/2024/6/untitled-ontology-41/>
PREFIX owl: <http://www.w3.org/2002/07/owl#>
PREFIX rdfs: <http://www.w3.org/2000/01/rdf-schema#>
PREFIX schema1: <http://schema.org/>
PREFIX skos: <http://www.w3.org/2004/02/skos/core#>
PREFIX xsd: <http://www.w3.org/2001/XMLSchema#>

<http://opengis.net/ont/geocode/>
    a owl:Ontology, skos:ConceptScheme ;
    skos:prefLabel "Geocoding Vocabulary"@en ;
    skos:definition "A vocabulary to define Geocoding systems within OGC" ;
.

<http://opengis.net/ont/geocode/GeoHash>
    a
        <http://opengis.net/ont/geocode/GeoHashCode> ,
        skos:Concept ;
.

<http://opengis.net/ont/geocode/OpenLocationCode>
    a
        <http://opengis.net/ont/geocode/GeoCode> ,
        skos:Concept ;
    skos:prefLabel "Open Location Code"@en ;
    schema1:citation "https://maps.google.com/pluscodes/"^^xsd:anyURI ;
    skos:altLabel "Plus Code"@en ;
    skos:definition "The Open Location Code is a geocode based on a system of regular grids. It may be used to identify any location on Earth." ;
.

<http://opengis.net/ont/geocode/What3Words>
    a
        <http://opengis.net/ont/geocode/GeoCode> ,
        skos:Concept ;
    skos:prefLabel "What3Words"@en ;
    skos:definition "What3Words is a proprietary Geocoding System by What3Words Limited that can be used to identify any  location on the surface of Earth within 3 metres." ;
.

:C-Squares
    a
        <http://opengis.net/ont/geocode/GeoCode> ,
        skos:Concept ;
    skos:prefLabel "C-Squares"@en ;
    skos:altLabel "Concise Spatial QUery And REpresentation System" ;
    schema1:citation "http://www.marine.csiro.au/csquares/"^^xsd:anyURI ;
    skos:definition "C-Squares is a system of spatially unique, location-based identifiers for areas on earth represented as cells from the Discrete Global Grid." ;
.

:CLLICode
    a
        <http://opengis.net/ont/geocode/GeoCode> ,
        skos:Concept ;
    skos:prefLabel "CLLI Code"@en ;
    skos:altLabel "Common Language Location Identifier Code"@en ;
    skos:definition "A location identifier code used within the North Amerian telecommunications industry to specify the location and function to telecommunications equipment" ;
.

:EirCode
    a
        :PostalCode ,
        skos:Concept ;
    skos:prefLabel "EirCode"@en ;
    skos:definition "Postal Code of Ireland"@en ;
.

:FIFACountryCode
    a
        :CountryCode ,
        skos:Concept ;
    skos:prefLabel "FIFA Country Code"@en ;
    skos:definition "The FIFA country code is a three-letter code to identify its member and non-member countries" ;
.

:GSSCode
    a
        :AdministrativeCode ,
        skos:Concept ;
    skos:prefLabel "GSS Code"@en ;
    skos:definition "A GSS Code is a nine-character geocode maintained by the United Kingdom's Office for National Statistics to represent geographical areas of the UK" ;
.

:GeoHash-36
    a
        <http://opengis.net/ont/geocode/GeoHashCode> ,
        skos:Concept ;
    skos:prefLabel "GeoHash-36"@en ;
    schema1:citation "https://web.archive.org/web/20121227195936/http://www.openpostcode.org/other-codes/geohash-36"^^xsd:anyURI ;
    skos:definition "GeoHash-36 is an open source compression algorithm for wolrd coordinate data" ;
.

:GeoRef
    a
        <http://opengis.net/ont/geocode/GeoCode> ,
        skos:Concept ;
    skos:prefLabel "GeoRef"@en ;
    schema1:citation "https://earth-info.nga.mil/GandG/coordsys/grids/georef.pdf"^^xsd:anyURI ;
    skos:altLabel "World Geographic Reference System"@en ;
.

:IANACountryCode
    a
        :CountryCode ,
        skos:Concept ;
    skos:prefLabel "IANA Country Code"@en ;
    skos:definition "The country codes which comprise the top level domain generally used by or reserved for a country" ;
.

:IATAAirportCode
    a
        :AirportCode ,
        skos:Concept ;
    skos:prefLabel "IATA Airport Code"@en ;
    skos:definition "A three-letter code issued by the International Air Transport Association (IATA) to identify airports and metropolitan areas on Earth." ;
.

:ICAOAirportCode
    a
        :AirportCode ,
        skos:Concept ;
    skos:prefLabel "ICAO Airport Code"@en ;
    skos:definition "A four-letter code used to identify aerodromes on Earth.";
.

:IOCCountryCode
    a
        :CountryCode ,
        skos:Concept ;
    skos:prefLabel "IOC Country Code"@en ;
    skos:definition "International Olympic Committee country codes identifying countries associated with the Olympic Games" ;
.

:ITU-RCountryCode
    a
        :CountryCode ,
        :TelephoneCode ,
        skos:Concept ;
    skos:prefLabel "ITU-R Country Code"@en ;
.

:ITU-TCountryCallingCode
    a
        :TelephoneCode ,
        skos:Concept ;
    skos:prefLabel "ITU-T Country Calling Code"@en ;
    skos:definition "Country calling codes are telephone number prefixes for reaching telephone subscribers in foreign countries or territories" ;
.

:ITU-TMobileCallingCode
    a
        :TelephoneCode ,
        skos:Concept ;
    skos:prefLabel "ITU-T Mobile Calling Code"@en ;
.

:MGRS
    a
        <http://opengis.net/ont/geocode/GeoCode> ,
        skos:Concept ;
    skos:prefLabel "MGRS"@en ;
    skos:altLabel "Military Grid Reference System"@en ;
    skos:definition "The geocoordinate standard derived from the UTM grid used by NATO militaries to located points on Earth." ;
.

:MaidenheadLocatorSystem
    a
        :AmateurRadio ,
        skos:Concept ;
    skos:prefLabel "Maidenhead Locator System"@en ;
    skos:altLabel
        "IARU Locator"@en ,
        "QTH Locator"@en ;
    skos:definition "Geocode System used by amateur radio operators"@en ;
.

:Mapcode
    a
        <http://opengis.net/ont/geocode/GeoCode> ,
        skos:Concept ;
    skos:prefLabel "Mapcode"@en ;
    schema1:citation "https://www.mapcode.com"^^xsd:anyURI ;
.

:MarsdenSquare
    a
        <http://opengis.net/ont/geocode/GeoCode> ,
        skos:Concept ;
    skos:prefLabel "Marsden Square"@en ;
    skos:definition "A system that divides a word map into a latitude-longitude grid" ;
.

:NaturalAddressCode
    a owl:Class ;
    skos:prefLabel "Natural Address Code"@en ;
    rdfs:subClassOf <http://opengis.net/ont/geocode/GeoCode> ;
.

:NaturalAreaCode
    a
        <http://opengis.net/ont/geocode/GeoCode> ,
        skos:Concept ;
    skos:prefLabel "Natural Area Code"@en ;
    schema1:citation "http://www.nacgeo.com"^^xsd:anyURI ;
    skos:altLabel "Universal Address"@en ;
    skos:definition "A proprietary geocode system for identifying areas anywhere on or in orbit around Earth." ;
.

:PlaceCode
    a owl:Class ;
    skos:prefLabel "Place Code"@en ;
    rdfs:subClassOf <http://opengis.net/ont/geocode/GeoCode> ;
    skos:altLabel "P-Code"@en ;
    skos:definition "A Geocode mostly used by emergency response teams"@en ;
.

:PostalndexNumber
    a
        :PostalCode ,
        skos:Concept ;
    skos:prefLabel "Postal Index Number"@en ;
    skos:definition "A six-digit code used by India Post" ;
.

:QRALocator
    a
        :AmateurRadio ,
        skos:Concept ;
    skos:prefLabel "QRA Locator"@en ;
    skos:altLabel "QTH Locator"@en ;
    skos:definition "Obsolete geocoding system used by amateur radio operators in Europe"@en ;
.

:UKPostCode
    a
        :PostalCode ,
        skos:Concept ;
    skos:prefLabel "UK PostCode"@en ;
    skos:definition "A postcode used to identify areas in the United Kingdom and its overseas territories" ;
.

:UN-LOCODE
    a
        <http://opengis.net/ont/geocode/GeoCode> ,
        skos:Concept ;
    skos:prefLabel "UN/LOCODE"@en ;
    schema1:citation "https://unece.org/trade/uncefact/unlocode"^^xsd:anyURI ;
    skos:altLabel "United Nations Code for Trade and Transport Locations"@en ;
.

:WMOSquare
    a
        <http://opengis.net/ont/geocode/GeoCode> ,
        skos:Concept ;
    skos:prefLabel "WMO Square"@en ;
    schema1:citation "https://www.nodc.noaa.gov/OC5/WOD05/data05geo.html"^^xsd:anyURI ;
    skos:altLabel "World Meteorological Organisation Square"@en ;
.

:ZIPCode
    a
        :PostalCode ,
        skos:Concept ;
    skos:prefLabel "ZIP Code"@en ;
    skos:definition "Postal Code of the USA"@en ;
.

<http://opengis.net/ont/geocode/GeoHashCode>
    a owl:Class ;
    skos:prefLabel "GeoHash Code"@en ;
    schema1:citation "http://geohash.org"^^xsd:anyURI ;
    rdfs:subClassOf <http://opengis.net/ont/geocode/GeoCode> ;
    skos:definition "A Geocode following the GeoHash encoding"@en ;
.

:AirportCode
    a owl:Class ;
    skos:prefLabel "Airport Code"@en ;
    skos:definition "A code used to identify the geolocation of an airport" ;
    rdfs:subClassOf <http://opengis.net/ont/geocode/GeoCode> ;
.

:AmateurRadio
    a owl:Class ;
    skos:prefLabel "Amateur radio"@en ;
    rdfs:subClassOf <http://opengis.net/ont/geocode/GeoCode> ;
    skos:definition "Geocodes used by operators in the amateur radio community"@en ;
.

:AdministrativeCode
    a owl:Class ;
    skos:prefLabel "Administrative Code"@en ;
    rdfs:subClassOf <http://opengis.net/ont/geocode/GeoCode> ;
.

:TelephoneCode
    a owl:Class ;
    skos:prefLabel "Telephone Code"@en ;
    skos:definition "A code used to identify telephones by location." ;
    rdfs:subClassOf <http://opengis.net/ont/geocode/GeoCode> ;
.

:CountryCode
    a owl:Class ;
    skos:prefLabel "Country Code"@en ;
    rdfs:subClassOf :AdministrativeCode ;
.

:PostalCode
    a owl:Class ;
    skos:prefLabel "Postal Code"@en ;
    rdfs:subClassOf :AdministrativeCode ;
.

<http://opengis.net/ont/geocode/GeoCode>
    a owl:Class ;
    skos:prefLabel "GeoCode"@en ;
.
