PREFIX dcterms: <http://purl.org/dc/terms/>
PREFIX geo: <http://www.opengis.net/ont/geosparql#>
PREFIX owl: <http://www.w3.org/2002/07/owl#>
PREFIX rdfs: <http://www.w3.org/2000/01/rdf-schema#>
PREFIX sdo: <https://schema.org/>
PREFIX sf: <http://www.opengis.net/ont/sf#>
PREFIX sf3d: <http://www.opengis.net/ont/sf3d#>
PREFIX skos: <http://www.w3.org/2004/02/skos/core#>
PREFIX xsd: <http://www.w3.org/2001/XMLSchema#>

sf3d:3DGeometry
    a
        rdfs:Class ,
        owl:Class ;
    rdfs:isDefinedBy <http://www.opengis.net/ont/sf3d> ;
    rdfs:subClassOf sf:Geometry ;
    skos:definition "A 3D geometry is a geometry that exclusively exists in at least 3 dimensions" ;
    skos:prefLabel "Cylinder"@en ;
.

sf3d:SolidGeometry
    a
        rdfs:Class ,
        owl:Class ;
    rdfs:isDefinedBy <http://www.opengis.net/ont/sf3d> ;
    rdfs:subClassOf sf3d:3DGeometry ;
    skos:definition "A solid geometry is a geometry that exists within a three-dimensional Euclidic Space." ;
    skos:prefLabel "solid geometry"@en ;
.


sf3d:Cylinder
    a
        rdfs:Class ,
        owl:Class ;
    rdfs:isDefinedBy <http://www.opengis.net/ont/sf3d> ;
    rdfs:subClassOf sf3d:SolidGeometry ;
    skos:definition """a solid geometrical figure with straight parallel sides and a circular or oval cross section"""@en ;
    skos:prefLabel "Cylinder"@en ;
.

sf3d:Cone
    a
        rdfs:Class ,
        owl:Class ;
    rdfs:isDefinedBy <http://www.opengis.net/ont/sf3d> ;
    rdfs:subClassOf sf3d:SolidGeometry ;
    skos:definition """a solid or hollow object which tapers from a circular or roughly circular base to a point"""@en ;
    skos:prefLabel "Cone"@en ;
.

sf3d:Texture
    a
        rdfs:Class ,
        owl:Class ;
    rdfs:isDefinedBy <http://www.opengis.net/ont/sf3d> ;
    rdfs:subClassOf sf:Polygon ;
    skos:definition """an image positioned on a defined position on the surface of a 3D solid"""@en ;
    skos:prefLabel "Texture"@en ;
.


sf3d:Face
    a
        rdfs:Class ,
        owl:Class ;
    rdfs:isDefinedBy <http://www.opengis.net/ont/sf3d> ;
    rdfs:subClassOf sf:Polygon ;
    skos:definition """a flat or curved surface on a 3D shape"""@en ;
    skos:prefLabel "Face"@en ;
.


sf3d:Pyramid
    a
        rdfs:Class ,
        owl:Class ;
    rdfs:isDefinedBy <http://www.opengis.net/ont/sf3d> ;
    rdfs:subClassOf sf3d:SolidGeometry ;
    skos:definition """a conic solid with a polygonal base."""@en ;
    skos:prefLabel "Pyramid"@en ;
.



sf3d:Torus
    a
        rdfs:Class ,
        owl:Class ;
    rdfs:isDefinedBy <http://www.opengis.net/ont/sf3d> ;
    rdfs:subClassOf sf3d:SolidGeometry ;
    skos:definition """a surface or solid formed by rotating a closed curve, especially a circle, about a line which lies in the same plane but does not intersect it"""@en ;
    skos:prefLabel "Torus"@en ;
.

sf3d:PointCloud
    a
        rdfs:Class ,
        owl:Class ;
    rdfs:isDefinedBy <http://www.opengis.net/ont/sf3d> ;
    rdfs:subClassOf sf3d:3DGeometry ;
    skos:definition """a set of points in threedimensional space"""@en ;
    skos:prefLabel "PointCloud"@en ;
.

sf3d:Mesh
    a
        rdfs:Class ,
        owl:Class ;
    rdfs:isDefinedBy <http://www.opengis.net/ont/sf3d> ;
    rdfs:subClassOf sf3d:3DGeometry ;
    skos:definition """ a structural build of a 3D model consisting of polygons"""@en ;
    skos:prefLabel "Mesh"@en ;
.

sf3d:Cube
    a
        rdfs:Class ,
        owl:Class ;
    rdfs:isDefinedBy <http://www.opengis.net/ont/sf3d> ;
    rdfs:subClassOf sf3d:SolidGeometry ;
    skos:definition """a symmetrical three-dimensional shape, either solid or hollow, contained by six equal squares"""@en ;
    skos:prefLabel "Cube"@en ;
.

sf3d:Cuboid
    a
        rdfs:Class ,
        owl:Class ;
    rdfs:isDefinedBy <http://www.opengis.net/ont/sf3d> ;
    rdfs:subClassOf sf3d:SolidGeometry ;
    skos:definition """a solid which has six rectangular faces at right angles to each other"""@en ;
    skos:prefLabel "Cuboid"@en ;
    skos:altLabel "Box"@en ;
.



sf3d:Boundary
    a
        rdfs:Class ,
        owl:Class ;
    rdfs:isDefinedBy <http://www.opengis.net/ont/sf3d> ;
    rdfs:subClassOf sf3d:SolidGeometry ;
    skos:definition """a round solid figure with every point on its surface equidistant from its centre"""@en ;
    skos:prefLabel "Boundary"@en ;
.


sf3d:Sphere
    a
        rdfs:Class ,
        owl:Class ;
    rdfs:isDefinedBy <http://www.opengis.net/ont/sf3d> ;
    rdfs:subClassOf sf3d:SolidGeometry ;
    skos:definition """a round solid figure with every point on its surface equidistant from its centre"""@en ;
    skos:prefLabel "Sphere"@en ;
.


sf3d:faces
    a
        rdfs:Class ,
        owl:Class ;
    rdfs:isDefinedBy <http://www.opengis.net/ont/sf3d> ;
    skos:definition """Relates a 3d solid to a face"""@en ;
    skos:prefLabel "faces"@en ;
    rdfs:range sf3d:Face ;
    rdfs:domain sf3d:SolidGeometry ;
. 

sf3d:textures
    a
        rdfs:Class ,
        owl:Class ;
    rdfs:isDefinedBy <http://www.opengis.net/ont/sf3d> ;
    skos:definition """Relates a 3d solid to a texture"""@en ;
    skos:prefLabel "textures"@en ;
    rdfs:range sf3d:Texture ;
    rdfs:domain sf3d:SolidGeometry ;
.


sf3d:matrixLiteral
    a
       rdf:Datatype ;
    rdfs:isDefinedBy <http://www.opengis.net/ont/sf3d> ;
    skos:definition """a projection matrix which can be applied to a 3D geometry"""@en ;
    skos:prefLabel "matrix literalBoundary"@en ;
.

<http://www.opengis.net/ont/sf3d>
    a owl:Ontology ;
    dcterms:creator "OGC GeoSPARQL Standards Working Group" ;
    dcterms:description "An RDF/OWL vocabulary for defining geometry types in 3D" ;
    dcterms:license "https://www.ogc.org/license"^^xsd:anyURI ;
    dcterms:modified "2022-06-16"^^xsd:date ;
    dcterms:publisher [
            a sdo:Organization ;
            sdo:name "Open Geospatial Consortium" ;
            sdo:url "https://www.ogc.org"^^xsd:anyURI
        ] ;
    dcterms:rights "(c) 2022 Open Geospatial Consortium" ;
    dcterms:title "Simple Features 3D Vocabulary" ;
    owl:versionIRI <http://www.opengis.net/ont/sf/1.3> ;
    owl:versionInfo "OGC GeoSPARQL 1.3" ;
.

